More WIP

ListADT.v
@@ -1,4 +1,4 @@
-Require Import String Omega List.
+Require Import String Omega.
 
 Generalizable All Variables.
 Set Implicit Arguments.
@@ -6,161 +6,162 @@ Set Implicit Arguments.
 
 (** * Basic ADT definitions *)
 
-(** Hoare logic-style total correctness specification of a mutator method *)
-Definition mutatorMethodSpec (Ty : Type) :=
+(** Hoare logic-style total correctness specification of a method *)
+Definition methodSpec (Ty : Type) :=
   Ty    (* Initial model *)
   -> nat (* Actual argument*)
   -> Ty (* Final model *)
-(*  -> nat (* Return value *) *)
-  -> Prop.
-
-(** Hoare logic-style total correctness specification of an obeserver method *)
-Definition observerMethodSpec (Ty : Type) :=
-  Ty    (* Initial model *)
-  -> nat (* Actual argument*)
-(*  -> Ty (* Final model *) *)
   -> nat (* Return value *)
   -> Prop.
 
 (** Interface of an ADT *)
-Record ADT :=
-  {
-    Model : Type;
-    (** The way we model state mathematically *)
+Record ADT := {
+  Model : Type;
+  (** The way we model state mathematically *)
 
-    MutatorIndex : Type;
-    (** The index set of mutators *)
+  MethodSpecs : string -> methodSpec Model
+  (** A specification for each method *)
+}.
 
-    ObserverIndex : Type;
-    (** The index set of observers *)
-
-    MutatorMethodSpecs : MutatorIndex -> mutatorMethodSpec Model;
-    (** A specification for each mutator method *)
-
-    ObserverMethodSpecs : ObserverIndex -> observerMethodSpec Model
-    (** A specification for each observer method *)
-  }.
 
 (** Implementation type of a method in Gallina *)
 Definition methodTypeD (State : Type) :=
   State -> nat -> State * nat.
 
-(** Usual Hoare logic notion of implementating a mutator method spec *)
-Definition mutatorMethodCorrect (Model State : Type) (ms : mutatorMethodSpec Model)
-           (RepInv : Model -> State -> Prop)
-           (mb : methodTypeD State)
-  := forall m s,
-       RepInv m s
-       -> forall x,
-            let s'y := mb s x in
-            exists m', RepInv m' (fst s'y)
-                       /\ ms m x m'
-                       /\ (snd s'y) = 0.
-
-Definition observerMethodCorrect (Model State : Type) (ms : observerMethodSpec Model)
-           (RepInv : Model -> State -> Prop)
-           (mb : methodTypeD State)
-  := forall m s,
-       RepInv m s
-       -> forall x,
-            let s'y := mb s x in
-            RepInv m (fst s'y)
-            /\ ms m x (snd s'y).
+(** Usual Hoare logic notion of implementating a method spec *)
+Definition methodCorrect (Model State : Type) (ms : methodSpec Model)
+  (RepInv : Model -> State -> Prop)
+  (mb : methodTypeD State) :=
+  forall m s, RepInv m s
+    -> forall x,
+      let (s', y) := mb s x in
+        exists m', RepInv m' s'
+          /\ ms m x m' y.
 
 (** One implementation of an ADT *)
-Record ADTimpl (A : ADT) :=
-  {
-    State : Type;
-    (** Real state type in Gallina *)
+Record ADTimpl (A : ADT) := {
+  State : Type;
+  (** Real state type in Gallina *)
 
-    RepInv : Model A -> State -> Prop;
-    (** Relationship between abstract (specification) and concrete (implementation) states *)
+  RepInv : Model A -> State -> Prop;
+  (** Relationship between abstract (specification) and concrete (implementation) states *)
 
-    MutatorMethodBodies : MutatorIndex A -> methodTypeD State;
-    (** An implementation of each mutator method *)
+  MethodBodies : string -> methodTypeD State;
+  (** An implementation of each method *)
 
-    ObserverMethodBodies : ObserverIndex A -> methodTypeD State;
-    (** An implementation of each observer method *)
-
-    MutatorMethodsCorrect : forall idx, mutatorMethodCorrect (MutatorMethodSpecs A idx)
-                                                             RepInv
-                                                             (MutatorMethodBodies idx);
-    (** All mutator methods satisfy their specs. *)
-
-    ObserverMethodsCorrect : forall idx, observerMethodCorrect (ObserverMethodSpecs A idx)
-                                                               RepInv
-                                                               (ObserverMethodBodies idx)
-    (** All observer methods satisfy their specs. *)
-  }.
+  MethodsCorrect : forall name, methodCorrect (MethodSpecs A name) RepInv
+    (MethodBodies name)
+  (** All methods satisfy their specs. *)
+}.
 
 
 (** * A simple pairing combinator *)
+
+(** When does a method spec force no state mutation? *)
+Definition observer Model (ms : methodSpec Model) :=
+  forall m x m' y, ms m x m' y
+    -> m = m'.
+
+(** When is a method not returning any data, but probably instead just causing side effects? *)
+Definition mutator Model (ms : methodSpec Model) :=
+  forall m x m' y, ms m x m' y
+    -> y = 0.
 
 Section paired.
   Variables A B : ADT.
   (** Let's compose these two ADTs. *)
 
-  Variable mutatorIndex : Type.
-  Variable observerIndex : Type.
-  Variable mutatorMap : mutatorIndex -> MutatorIndex A * MutatorIndex B.
-  Variable observerMap : observerIndex -> ObserverIndex A + ObserverIndex B.
+  (** We'll want to classify each method as follows: *)
+  Inductive methodSort :=
+  | ObserverA (* Observer implemented by [A] *)
+  | ObserverB (* Observer implemented by [B] *)
+  | Mutator   (* Mutator implemented by _both_ *)
+  | Dummy     (* Just gets a dummy implementation in composition *).
+
+  (** When is one of these classifications accurate? *)
+  Definition methodSort_accurate (s : methodSort) (name : string) :=
+    match s with
+      | ObserverA => observer (MethodSpecs A name)
+      | ObserverB => observer (MethodSpecs B name)
+      | Mutator => mutator (MethodSpecs A name) /\ mutator (MethodSpecs B name)
+      | Dummy => True
+    end.
+
+  (** Require client code to classify the methods for us. *)
+  Variable sortOf : string -> methodSort.
 
   (** The composed ADT *)
-  Program Definition pairedADT :=
+  Definition pairedADT :=
     {|
       Model := Model A * Model B;
-      MutatorIndex := mutatorIndex;
-      ObserverIndex := observerIndex;
-      MutatorMethodSpecs idx := let s := mutatorMap idx in
-                                fun m x m' => MutatorMethodSpecs A (fst s) (fst m) x (fst m')
-                                              /\ MutatorMethodSpecs B (snd s) (snd m) x (snd m');
-      ObserverMethodSpecs idx := fun m => match observerMap idx with
-                                            | inl idx' => ObserverMethodSpecs A idx' (fst m)
-                                            | inr idx' => ObserverMethodSpecs B idx' (snd m)
-                                          end
+      MethodSpecs := fun name => match sortOf name with
+                                   | ObserverA
+                                     => fun m x m' y
+                                        => MethodSpecs A name (fst m) x (fst m') y
+                                   | ObserverB
+                                     => fun m x m' y
+                                        => MethodSpecs B name (snd m) x (snd m') y
+                                   | Mutator
+                                     => fun m x m' y
+                                        => MethodSpecs A name (fst m) x (fst m') y
+                                           /\ MethodSpecs B name (snd m) x (snd m') y
+                                   | _ => fun _ _ _ _ => True
+                                 end
     |}.
 
   (** Now we show how to implement it. *)
   Variable Ai : ADTimpl A.
   Variable Bi : ADTimpl B.
 
+  Local Hint Extern 1 (@ex (_ * _) _) => eexists (_, _).
+
+  Hypothesis sortOf_accurate : forall name, methodSort_accurate (sortOf name) name.
+
   Definition pairedImpl : ADTimpl pairedADT.
-  Proof.
     refine {|
-        State := State Ai * State Bi;
-        RepInv := fun (m : Model pairedADT) s => RepInv Ai (fst m) (fst s)
-                                                 /\ RepInv Bi (snd m) (snd s);
-        MutatorMethodBodies name := fun s x => ((fst (MutatorMethodBodies Ai (fst (mutatorMap name)) (fst s) x),
-                                                 fst (MutatorMethodBodies Bi (snd (mutatorMap name)) (snd s) x)),
-                                                0);
-        ObserverMethodBodies name := fun s x => match observerMap name with
-                                                  | inl name' => let sy := ObserverMethodBodies Ai name' (fst s) x in
-                                                                 ((fst sy, snd s), snd sy)
-                                                  | inr name' => let sy := ObserverMethodBodies Bi name' (snd s) x in
-                                                                 ((fst s, fst sy), snd sy)
-                                                end
-      |};
-    repeat match goal with
-             | _ => intro
-             | _ => progress simpl in *
-             | [ idx : mutatorIndex, H : RepInv Ai _ _ /\ RepInv Bi _ _, x : nat |- _ ]
-               => generalize (MutatorMethodsCorrect Ai (fst (mutatorMap idx)) _ _ (proj1 H) x);
-                 generalize (MutatorMethodsCorrect Bi (snd (mutatorMap idx)) _ _ (proj2 H) x);
-                 destruct (mutatorMap idx), H; simpl in *;
-                 clear idx;
-                 progress repeat destruct MutatorMethodBodies;
-                 firstorder; subst
-             | [ idx : observerIndex |- _ ]
-               => destruct (observerMap idx) as [idx'|idx']; clear idx
-             | _ => eexists (_, _)
-             | _ => progress (repeat esplit; try eassumption)
-             | _ => apply ObserverMethodsCorrect
-             | _ => progress firstorder intuition
-           end.
+      State := State Ai * State Bi;
+      RepInv := fun (m : Model pairedADT) s => RepInv Ai (fst m) (fst s)
+        /\ RepInv Bi (snd m) (snd s);
+      MethodBodies := fun name => match sortOf name as s with
+                                    | ObserverA => fun s x =>
+                                      let (s', y) := MethodBodies Ai name (fst s) x in
+                                        ((s', snd s), y)
+                                    | ObserverB => fun s x =>
+                                      let (s', y) := MethodBodies Bi name (snd s) x in
+                                        ((fst s, s'), y)
+                                    | Mutator => fun s x =>
+                                      let (s1, _) := MethodBodies Ai name (fst s) x in
+                                        let (s2, _) := MethodBodies Bi name (snd s) x in
+                                          ((s1, s2), 0)
+                                    | Dummy => fun s _ => (s, 0)
+                                  end
+    |}.
+
+    simpl; intros name.
+    generalize (sortOf_accurate name).
+    destruct (sortOf name); simpl; unfold observer, mutator, methodCorrect;
+    (simpl; intuition; simpl in *).
+
+    - specialize (MethodsCorrect Ai name a (fst s) H1 x); simpl; intuition.
+      destruct MethodBodies; firstorder eauto 10.
+
+    - specialize (MethodsCorrect Bi name b (snd s) H2 x); simpl; intuition.
+      destruct MethodBodies; firstorder eauto 10.
+
+    - specialize (MethodsCorrect Ai name a (fst s) H2 x); simpl; intuition.
+      destruct MethodBodies; firstorder.
+      specialize (MethodsCorrect Bi name b (snd s) H3 x); simpl; intuition.
+      destruct MethodBodies; firstorder.
+      eexists (_, _); simpl.
+      repeat esplit; simpl; eauto.
+      replace 0 with n; eauto.
+      replace 0 with n0; eauto.
+
+    - eauto.
   Defined.
 End paired.
 
-(*
+
 
 Section prod.
   Variable model : Type.
@@ -168,11 +169,6 @@ Section prod.
 
   Let A := {| Model := model; MethodSpecs := ASpec |}.
   Let B := {| Model := model; MethodSpecs := BSpec |}.
-
-  Variable mutatorIndex : Type.
-  Variable observerIndex : Type.
-  Variable mutatorMap : mutatorIndex -> MutatorIndex A * MutatorIndex B.
-  Variable observerMap : observerIndex -> ObserverIndex A + ObserverIndex B.
 
   (** Let's compose these two ADTs. *)
 
@@ -248,7 +244,7 @@ Section prod.
     generalize (sortOf_accurate name).
     generalize (mutators_match name).
     destruct (sortOf name); simpl; unfold observer, mutator, methodCorrect, methods_match_mutation;
-      (simpl; intuition; simpl in * );
+      (simpl; intuition; simpl in *);
       match goal with
         | [ H1 : RepInv Ai m (fst s), H2 : RepInv Bi m (snd s) |- _ ]
           => specialize (MethodsCorrect Ai name m (fst s) H1 x);
@@ -263,7 +259,7 @@ Section prod.
                 | repeat esplit; [ | eassumption | ]; fin_tac ].
   Defined.
 End prod.
-*)
+
 (** * An example, composing binary commutative associative calculators for computable nat multisets *)
 
 Definition multiset := nat -> nat.
@@ -273,7 +269,7 @@ Definition add (s : multiset) (n : nat) : multiset
               else s m.
 
 Require Import Min Max List.
-(*
+
 Fixpoint make_specs model (spec_list : list (string * methodSpec model))
   := fun s
      => match spec_list with
@@ -302,7 +298,6 @@ Definition make_accessor
         /\ f n d n'.
 
 Arguments make_accessor / .
-*)
 
 Coercion sumbooltobool A B : {A} + {B} -> bool := fun x => if x then true else false.
 
@@ -313,28 +308,32 @@ Infix ">" := gt_dec : bool_scope.
 Infix "->" := implb : bool_scope.
 
 Definition NatBinOp
+           (addname : string)
+           (opname : string)
            (op : nat -> nat -> nat)
            (is_assoc : forall x y z, op x (op y z) = op (op x y) z)
            (is_comm : forall x y, op x y = op y x)
-           (default_value : nat)
 : ADT
   := {|
       Model := multiset;
-      MutatorIndex := unit;
-      ObserverIndex := unit;
-      MutatorMethodSpecs u m x m' := forall k, m' k = (add m x) k;
-      ObserverMethodSpecs u m x n := exists l : list nat,
-                                       (forall v, m v = count_occ eq_nat_dec l v)
-                                       /\ match l with
-                                            | nil => n = default_value
-                                            | cons z zs => n = fold_right op z zs
-                                          end
+      MethodSpecs :=
+        make_specs ((opname,
+                     make_accessor (fun _ (m : multiset) n
+                                    => exists l : list nat,
+                                         (forall v, m v = count_occ eq_nat_dec l v)
+                                         /\ match l with
+                                              | nil => True
+                                              | cons x xs => n = fold_right op x xs
+                                            end))
+                      ::common_multiset_specs addname)
     |}.
 
 Local Ltac rewrite_hyp' :=
   match goal with
     | [ H : _ |- _ ] => rewrite H
   end.
+
+Require Import Omega.
 
 Local Obligation Tactic :=
   eauto with arith;
@@ -344,17 +343,17 @@ Local Obligation Tactic :=
                      end
             | intros; omega ].
 
-Program Definition NatLower default_value : ADT
-  := NatBinOp min _ _ default_value.
+Program Definition NatLower addName lowerBoundName : ADT
+  := NatBinOp addName lowerBoundName min _ _.
 
-Program Definition NatUpper default_value : ADT
-  := NatBinOp max _ _ default_value.
+Program Definition NatUpper addName upperBoundName : ADT
+  := NatBinOp addName upperBoundName max _ _.
 
-Program Definition NatSum default_value : ADT
-  := NatBinOp plus _ _ default_value.
+Program Definition NatSum addName sumName : ADT
+  := NatBinOp addName sumName plus _ _.
 
-Program Definition NatProd default_value : ADT
-  := NatBinOp mult _ _ default_value.
+Program Definition NatProd addName prodName : ADT
+  := NatBinOp addName prodName mult _ _.
 
 
 Hint Immediate le_min_l le_min_r le_max_l le_max_r.
@@ -372,6 +371,8 @@ Lemma max_trans : forall n m v,
 Qed.
 
 Hint Resolve min_trans max_trans.
+
+Require Import FunctionalExtensionality.
 
 Arguments add _ _ _ / .
 
@@ -435,6 +436,7 @@ Section def_NatBinOpI.
              | [ H : appcontext[match ?x with _ => _ end] |- _  ] => destruct x
              | [ H : Some _ = Some _ |- _ ] => inversion H; clear H
              | _ => progress f_equal; []
+             | _ => apply functional_extensionality_dep; intro
              | _ => progress intuition
              | _ => repeat esplit; reflexivity
              | [ H : _ |- _ ] => rewrite H; try (rewrite H; fail 1)
@@ -444,31 +446,45 @@ Section def_NatBinOpI.
     repeat first [ progress t
                  | progress induction_list_then ltac:(solve_after_induction_list op op_assoc op_comm) ].
 
-  Definition NatBinOpI
-  : `(ADTimpl (@NatBinOp op op_assoc op_comm default_value)).
+  Definition NatBinOpI (default_val : nat) addname opname (H : if string_dec addname opname then False else True)
+  : `(ADTimpl (@NatBinOp addname opname op op_assoc op_comm)).
   Proof.
     intros.
     refine {|
         State := option nat;
-        RepInv := fun (m : Model (NatBinOp op op_assoc op_comm default_value)) n
+        RepInv := fun (m : Model (NatBinOp addname opname op op_assoc op_comm)) n
                   => exists l : list nat,
                        (forall v, m v = count_occ eq_nat_dec l v)
                        /\ match l with
                             | nil => n = None
                             | cons x xs => n = Some (fold_right op x xs)
                           end;
-        MutatorMethodBodies u val x := (match val with
-                                          | None => Some x
-                                          | Some x' => Some (op x x')
-                                        end,
-                                        0);
-        ObserverMethodBodies u val x := (val,
-                                         match val with
-                                           | None => default_value
-                                           | Some x => x
-                                         end)
-      |};
-      intros [];
+        MethodBodies := fun s =>
+                          if string_dec s addname
+                          then fun val x => (match val with
+                                               | None => Some x
+                                               | Some x' => Some (op x x')
+                                             end,
+                                             0)
+                          else if string_dec s opname
+                               then fun val _ => (val,
+                                                  match val with
+                                                    | None => default_val
+                                                    | Some x => x
+                                                  end)
+                               else fun val _ => (val, 0)
+      |}.
+    intro name.
+    simpl.
+    repeat match goal with
+             | [ H : False |- _ ] => destruct H
+             | [ H : ?x <> ?x |- _ ] => destruct (H eq_refl)
+             | [ H : ?x = ?x -> False |- _ ] => destruct (H eq_refl)
+             | [ |- appcontext[if ?E then _ else _] ] => let H := fresh "H'0" in
+                                                         destruct E as [H|H]; subst
+             | [ H : appcontext[if ?E then _ else _] |- _ ] => let H := fresh "H'0" in
+                                                               destruct E as [H|H]; subst
+           end;
       try solve [intros m [n|] [l [H0 H1]] x;
                   (exists (add m x));
                   repeat split;
@@ -492,45 +508,19 @@ Section def_NatBinOpI.
   Defined.
 End def_NatBinOpI.
 
-Definition NatLowerI default_val : ADTimpl (NatLower default_val)
-  := NatBinOpI _ _ _ _.
+Definition NatLowerI addName lowerBoundName H : ADTimpl (NatLower addName lowerBoundName)
+  := NatBinOpI 0 addName lowerBoundName H _ _ _.
 
-Definition NatUpperI default_val : ADTimpl (NatUpper default_val)
-  := NatBinOpI _ _ _ _.
+Definition NatUpperI addName upperBoundName H : ADTimpl (NatUpper addName upperBoundName)
+  := NatBinOpI 0 addName upperBoundName H _ _ _.
 
-Definition NatSumI default_val : ADTimpl (NatSum default_val)
-  := NatBinOpI _ _ _ _.
+Definition NatSumI addName sumName H : ADTimpl (NatSum addName sumName)
+  := NatBinOpI 0 addName sumName H  _ _ _.
 
-Definition NatProdI default_val : ADTimpl (NatProd default_val)
-  := NatBinOpI _ _ _ _.
+Definition NatProdI addName prodName H : ADTimpl (NatProd addName prodName)
+  := NatBinOpI 1 addName prodName H _ _ _.
 
 Local Open Scope string_scope.
-
-Definition NatSumProd_spec : ADT
-  := {| Model := multiset * multiset;
-        MutatorIndex := unit;
-        ObserverIndex := unit + unit;
-        MutatorMethodSpecs u m x m' := (forall k, (fst m') k = (add (fst m) x) k)
-                                       /\ (forall k, (snd m') k = (add (snd m) x) k);
-        ObserverMethodSpecs u m x n := match u with
-                                         | inl _ => exists l : list nat,
-                                                      (forall v, (fst m) v = count_occ eq_nat_dec l v)
-                                                      /\ match l with
-                                                           | nil => n = 0
-                                                           | cons z zs => n = fold_right plus z zs
-                                                         end
-                                         | inr _ => exists l : list nat,
-                                                      (forall v, (snd m) v = count_occ eq_nat_dec l v)
-                                                      /\ match l with
-                                                           | nil => n = 1
-                                                           | cons z zs => n = fold_right mult z zs
-                                                         end
-                                       end
-     |}.
-
-Goal ADTimpl NatSumProd_spec.
-Print pairedImpl.
-eapply pairedImpl.
 
 Definition NatLowerUpper_sortOf (s : string) :=
   if string_dec s "add"
